verification/theories/memory_tracker/page_allocator/page_allocator_extra.v
@@ -1,5 +1,53 @@
 From refinedrust Require Import typing.
+From refinedrust Require Import ghost_var_dfrac.
 From ace.theories.page Require Import page_extra.
+
+(** * Page allocator ghost state *)
+Record memory_region := {
+  mreg_start : Z;
+  mreg_size : nat;
+}.
+Definition mreg_end (mreg : memory_region) : Z :=
+  mreg.(mreg_start) + mreg.(mreg_size).
+
+(*Definition memory_region_incl *)
+
+Class memory_regionG Σ := {
+  mreg_ghost_var :: ghost_varG Σ memory_region;
+}.
+Section page_allocator.
+  Context `{!typeGS Σ}.
+  Context `{!memory_regionG Σ}.
+  
+  Definition has_memory_region_def (γ : gname) (mreg : memory_region) :=
+    ghost_var γ DfracDiscarded mreg.
+  Definition has_memory_region_aux : seal (@has_memory_region_def). Proof. by eexists. Qed.
+  Definition has_memory_region := has_memory_region_aux.(unseal).
+  Definition has_memory_region_eq : @has_memory_region = @has_memory_region_def := has_memory_region_aux.(seal_eq).
+
+  Lemma has_memory_region_alloc mreg : 
+    ⊢ |==> ∃ γ, has_memory_region γ mreg.
+  Proof.
+    rewrite has_memory_region_eq.
+    iMod (ghost_var_alloc mreg) as (γ) "Hvar".
+    iExists γ. by iApply ghost_var_discard.
+  Qed.
+
+  Lemma has_memory_region_agree γ mreg1 mreg2 :
+    has_memory_region γ mreg1 -∗
+    has_memory_region γ mreg2 -∗
+    ⌜mreg1 = mreg2⌝.
+  Proof.
+    rewrite has_memory_region_eq.
+    iApply ghost_var_agree.
+  Qed.
+
+  Global Instance has_memory_region_pers γ mreg : Persistent (has_memory_region γ mreg).
+  Proof.
+    rewrite has_memory_region_eq.
+    apply _.
+  Qed.
+End page_allocator.
 
 (*
 (** [m1] is a correct abstraction of [m2] to only specify the number of pages at a given size. *)
@@ -14,10 +62,15 @@ Definition page_allocator_maps_related (m1 : gmap page_size nat) (m2 : gmap page
       Forall (λ pg : page, pg.(page_sz) = sz) list_pages.
 *)
 
+(** * Page allocator invariants *)
 Inductive node_allocation_state :=
+
   | PageNodeUnavailable
+
   | PageNodeAvailable
-  | PageNodePartiallyAvailable
+
+  | PageNodePartiallyAvailable (allocable_sz : page_size)
+
 .
 
 Global Instance node_allocation_state_eqdec : EqDecision node_allocation_state.
@@ -31,8 +84,10 @@ Record page_storage_node : Type := mk_page_node {
   max_node_size : page_size;
   (* The base address of the memory region of this node *)
   base_address : Z;
-  
+  (* the current state of this node *)
   allocation_state : node_allocation_state;
+  (* whether the child nodes have been initialized *)
+  children_initialized : bool;
 }.
 
 (** Compute the base address of a child node *)
@@ -55,40 +110,66 @@ Definition page_storage_node_children_wf (parent_base_address : Z) (parent_node_
     children = [])
 .
 
+Definition page_node_can_allocate (node : page_storage_node) : option page_size := 
+  match node.(allocation_state) with
+  | PageNodeUnavailable => None
+  | PageNodeAvailable => Some node.(max_node_size)
+  | PageNodePartiallyAvailable allocable => Some allocable
+  end.
+
 
 Definition page_storage_node_invariant
   (node : page_storage_node)
   (max_sz : option page_size) (maybe_page_token : option page) (children : list page_storage_node) :=
+
   (* The children, if any, are well-formed *)
   page_storage_node_children_wf node.(base_address) node.(max_node_size) children ∧
   (* the base address is suitably aligned *)
   (page_size_align node.(max_node_size) | node.(base_address))%Z ∧
+
+  (* initialization of child nodes *)
+  (if node.(children_initialized) then length children = page_size_multiplier node.(max_node_size) else True) ∧
+
   (* invariant depending on the allocation state: *)
   if decide (node.(allocation_state) = PageNodeUnavailable) 
   then 
       (* No allocation is possible *)
-      maybe_page_token = None ∧ max_sz = None
+      maybe_page_token = None ∧ max_sz = None ∧
+
+      (* all children are unavailable *)
+      (* TODO do we need this *)
+      Forall (λ child, child.(allocation_state) = PageNodeUnavailable) children
   else if decide (node.(allocation_state) = PageNodeAvailable)
   then
       (* This node is completely available *) 
       ∃ token,
         (* there is some token *)
         maybe_page_token = Some token ∧
+        (* the allocable size spans the whole page *)
+        max_sz = Some (node.(max_node_size)) ∧
         (* the token spans the whole node *)
         token.(page_loc).2 = node.(base_address) ∧
         token.(page_sz) = node.(max_node_size) ∧
-        (* the allocable size spans the whole page *)
-        max_sz = Some (node.(max_node_size)) ∧
+        
         (* all children are unavailable *)
+        (* TODO: do we need this? *)
         Forall (λ child, child.(allocation_state) = PageNodeUnavailable) children
   else 
+
       (* This node is partially available with initialized children *)
       maybe_page_token = None ∧
-      length children = page_size_multiplier node.(max_node_size) ∧
+      (* Some size is available *)
+      ∃ allocable_sz, 
+      node.(allocation_state) = PageNodePartiallyAvailable allocable_sz ∧
+      max_sz = Some allocable_sz ∧
+      
+      (* children need to be initialized *)
+      node.(children_initialized) = true ∧
+
       (* The maximum size stored in this node needs to be available in one of the children *)
       ∃ i child, 
         children !! i = Some child ∧ 
-        child.(allocation_state) = PageNodeAvailable
+        page_node_can_allocate child = Some allocable_sz
 .
 
 Lemma page_storage_node_invariant_empty node_size base_address :
@@ -96,14 +177,10 @@ Lemma page_storage_node_invariant_empty node_size base_address :
   page_storage_node_invariant (mk_page_node node_size base_address PageNodeUnavailable) None None [].
 Proof.
   intros.
-  split_and!; simpl; [ | done..].
-  split; done.
+  split_and!; simpl; last split_and!; try done.
+  apply Nat2Z.divide. done.
 Qed.
 
-
-
-
+(* TODO unify all the memory range stuff *)
 Definition page_within_range (base_address : Z) (sz : page_size) (p : page) : Prop :=
-  base_address ≤ p.(page_loc).2 ∧ p.(page_loc).2 + page_size_in_bytes_Z p.(page_sz) < base_address + page_size_in_bytes_Z sz.
-      
-  
+  (base_address ≤ p.(page_loc).2 ∧ p.(page_loc).2 + page_size_in_bytes_Z p.(page_sz) < base_address + page_size_in_bytes_Z sz)%Z.
